filled in the proof of various lemmas

heap.lean
@@ -1,14 +1,16 @@
 import data.bitvec
 import data.dlist
+import data.list.perm
 import util.logic
 import util.control.applicative
 import util.control.monad.non_termination
 import util.data.option
 import util.meta.tactic
+import util.meta.tactic.perm
 
 universes u v w w'
 
-open nat list function
+open nat list (hiding bind) function
 
 @[reducible]
 def pointer := ℕ
@@ -37,13 +39,28 @@ if p = q then some v else none
 def heap.emp : heap :=
 λ _, none
 
+@[simp]
 lemma heap_emp_disjoint (h : heap)
 : heap.emp ## h :=
-by { unfold disjoint heap.emp, intros, left, refl }
+by { dunfold disjoint heap.emp, intros, left, refl }
 
 @[simp]
-lemma heap_emp_part_eq_self (h : heap)
+lemma disjoint_heap_emp (h : heap)
+: h ## heap.emp :=
+by { dunfold disjoint heap.emp, intros, right, refl }
+
+@[simp]
+lemma heap_emp_part'_eq_self (h : heap)
 : part' heap.emp h (heap_emp_disjoint _) = h :=
+begin
+  apply funext, intro,
+  unfold part',
+  cases (h x) ; simp [heap.emp,has_orelse.orelse,option.orelse]
+end
+
+@[simp]
+lemma part'_heap_emp_eq_self (h : heap)
+: part' h heap.emp (disjoint_heap_emp _) = h :=
 begin
   apply funext, intro,
   unfold part',
@@ -76,6 +93,17 @@ else none
 
 end noncomp
 
+@[simp]
+lemma heap_emp_part (h : heap)
+: part heap.emp h = some h :=
+by simp [part]
+
+@[simp]
+lemma part_heap_emp (h : heap)
+: part h heap.emp = some h :=
+by simp [part]
+
+@[symm]
 lemma disjoint_symm {h₀ h₁ : heap}
   (h : h₀ ## h₁)
 : h₁ ## h₀ :=
@@ -112,7 +140,7 @@ begin
   { assumption }
 end
 
-lemma part_disjoint_assoc {h₀ h₁ h₂ : heap}
+lemma part_disjoint_assoc_left {h₀ h₁ h₂ : heap}
   (Hdisj : h₀ ## h₁)
   (Hdisj' : h₁ ## h₂)
   (h : part' h₀ h₁ Hdisj ## h₂)
@@ -125,21 +153,59 @@ begin
   { simp [h',Hdisj p], },
 end
 
+lemma part_disjoint_assoc_right {h₀ h₁ h₂ : heap}
+  (Hdisj : h₀ ## h₁)
+  (Hdisj' : h₁ ## h₂)
+  (h : h₀ ## part' h₁ h₂)
+: part' h₀ h₁ ## h₂ :=
+begin
+  intro p,
+  cases h p with h' h' ; unfold part' at *,
+  { simp [h',Hdisj' p], },
+  { rw or_else_eq_none_iff at h',
+    simp [h'.right] },
+end
+
+@[simp]
+lemma eq_emp_of_part' (hp a : heap)
+  (h  : a ## hp)
+: a = part' a hp ↔ hp = heap.emp :=
+sorry
+
+@[simp]
+lemma eq_emp_of_part (hp a : heap)
+: some a = part a hp ↔ hp = heap.emp :=
+sorry
+
+@[simp]
+lemma part'_eq_emp (a b : heap)
+  (h  : a ## b)
+: part' a b = heap.emp ↔ a = heap.emp ∧ b = heap.emp :=
+sorry
+
+lemma part'_part'_assoc {h₀ h₁ h₂ : heap}
+  (Hdisj₀ : h₀ ## h₁)
+  (Hdisj₁ : h₁ ## h₂)
+  (Hdisj₂ : part' h₀ h₁ ## h₂)
+  (Hdisj₃ : h₀ ## part' h₁ h₂)
+: part' (part' h₀ h₁) h₂ Hdisj₂ = part' h₀ (part' h₁ h₂) Hdisj₃ :=
+sorry
+
 lemma part'_part_assoc {h₀ h₁ h₂ : heap}
-  (Hdisj : disjoint h₀ h₁)
-  (Hdisj' : disjoint h₁ h₂)
+  (Hdisj : h₀ ## h₁)
+  (Hdisj' : h₁ ## h₂)
 : part (part' h₀ h₁) h₂ = part h₀ (part' h₁ h₂) :=
 begin
   unfold part,
   cases classical.em (part' h₀ h₁ Hdisj ## h₂) with h h,
-  { have h' : (h₀ ## part' h₁ h₂ Hdisj') := part_disjoint_assoc _ _ h,
+  { have h' : (h₀ ## part' h₁ h₂ Hdisj') := part_disjoint_assoc_left _ _ h,
     simp [dif_pos,h,h'],
     apply congr_arg,
     funext p, simp [part',or_else_assoc], },
   { have h' : ¬ (h₀ ## part' h₁ h₂ Hdisj'),
     { rw part_comm',
       apply mt disjoint_symm,
-      apply mt (part_disjoint_assoc _ _),
+      apply mt (part_disjoint_assoc_left _ _),
       apply mt disjoint_symm,
       rw part_comm',
       apply h,
@@ -156,7 +222,47 @@ begin
   injection H_1,
 end
 
-lemma disjoint_disjoint {h₁ h₂ h₃ : heap}
+def heap.le (hp₀ hp₁ : heap) : Prop :=
+∃ hp, some hp₁ = part hp₀ hp
+
+instance : has_le heap :=
+⟨ heap.le ⟩
+
+instance : partial_order heap :=
+{ le := heap.le
+, le_refl := by { intro x, existsi heap.emp, simp [part_comm] }
+, le_trans := by { introv,
+                   simp [has_le.le,heap.le],
+                   intros hp₀ h₀ hp₁ h₁,
+                   have : hp₀ ## hp₁, admit,
+                   existsi part' hp₀ hp₁,
+                   rw [h₁,part'_of_part h₀,part'_part_assoc], }
+, le_antisymm := by { introv,
+                      simp [has_le.le,heap.le],
+                      intros hp₀ h₀ hp₁ h₁,
+                      have h : hp₀ ## hp₁, admit,
+                      rw [part'_of_part h₀,part'_part_assoc _ h
+                         ,eq_emp_of_part,part'_eq_emp] at h₁,
+                      simp [h₁.left] at h₀,
+                      injection h₀, subst b, }
+}
+
+lemma part'_delete_maplet (p : pointer) (v : word) (hp : heap)
+  (h : heap.delete p 1 hp ## maplet p v)
+  (h' : maplet p v ≤ hp)
+: part' (heap.delete p 1 hp) (maplet p v) = hp :=
+begin
+  funext p',
+  by_cases (p = p') with h,
+  { simp [part', heap.delete, maplet, if_pos, h],
+    unfold has_le.le heap.le at h',
+    cases h' with hp' h',
+    rw [part'_of_part h',part',maplet,if_pos h],
+    simp },
+  { simp [part', heap.delete, maplet, if_neg, h] }
+end
+
+lemma disjoint_disjoint_left {h₁ h₂ h₃ : heap}
   (H₁ : h₂ ## h₃)
   (H₀ : part' h₂ h₃ H₁ ## h₁)
 : h₁ ## h₃ :=
@@ -168,3 +274,145 @@ begin
     simp [H₂.right] },
   { simp [H₂] }
 end
+
+lemma disjoint_disjoint_right {h₁ h₂ h₃ : heap}
+  (H₁ : h₂ ## h₃)
+  (H₀ : part' h₂ h₃ H₁ ## h₁)
+: h₁ ## h₂ :=
+begin
+  have H₁ := disjoint_symm H₁,
+  apply disjoint_disjoint_left H₁,
+  rw part_comm', apply H₀,
+end
+
+noncomputable def parts : list heap → option heap
+ | [] := some heap.emp
+ | (x :: xs) :=
+do ys ← parts xs,
+   part x ys
+
+lemma parts_congr {hp₀ hp₁ : list heap}
+  (H : hp₀ ~ hp₁)
+: parts hp₀ = parts hp₁ :=
+begin
+  induction H,
+  case perm.nil
+  { refl },
+  case perm.skip
+  { unfold parts,
+    rw ih_1, },
+  case perm.swap
+  { unfold parts,
+    simp [monad.bind_assoc],
+    apply congr_arg,
+    funext z,
+    unfold part,
+    cases classical.em (disjoint x z) with h h
+    ; cases classical.em (disjoint y z) with h' h'
+    ; simp [h,h']
+    ; simp [bind,option.bind],
+    { rw [part_comm',← part'_part_assoc h',part_comm], },
+    { unfold part,
+      rw dif_neg, intros h'', apply h',
+      apply disjoint_disjoint_left,
+      symmetry, assumption },
+    { unfold part,
+      rw dif_neg, intros h'', apply h,
+      apply disjoint_disjoint_left,
+      symmetry, assumption },  },
+  case perm.trans
+  { cc }
+end
+
+lemma part'_eq_parts_app_of_parts_parts {hp₀ hp₁ : heap} {hs₀ hs₁ : list heap}
+  (H₀ : hp₀ ## hp₁)
+  (H₁ : some hp₀ = parts hs₀)
+  (H₂ : some hp₁ = parts hs₁)
+: some (part' hp₀ hp₁) = parts (hs₀ ++ hs₁) :=
+sorry
+
+lemma part_eq_parts_app_of_parts_parts {hp₀ hp₁ : heap} {hs₀ hs₁ : list heap}
+  (H₁ : some hp₀ = parts hs₀)
+  (H₂ : some hp₁ = parts hs₁)
+: part hp₀ hp₁ = parts (hs₀ ++ hs₁) :=
+sorry
+
+lemma parts_singleton (hp : heap)
+: some hp = parts [hp] :=
+sorry
+
+namespace tactic.interactive
+
+open tactic
+
+/-- Given `h : heap`, find `hs : list heap` such that `some h = parts hs` -/
+meta def flat_heap_expr : expr → tactic (dlist expr × expr)
+ | `(part' %%h₀ %%h₁ %%Hd) :=
+do (hs₀,p₀) ← flat_heap_expr h₀,
+   (hs₁,p₁) ← flat_heap_expr h₁,
+   p ← to_expr ``(part'_eq_parts_app_of_parts_parts %%Hd %%p₀ %%p₁),
+   return (hs₀ ++ hs₁,p)
+ | h :=
+do p ← to_expr ``(parts_singleton %%h),
+   return (dlist.singleton h, p )
+
+/-- Given `h : option heap`, find `hs : list heap` such that `h = parts hs` -/
+meta def flat_opt_heap_expr : expr → tactic (dlist expr × expr)
+ | `(part %%h₀ %%h₁) :=
+do (hs₀,p₀) ← flat_heap_expr h₀,
+   (hs₁,p₁) ← flat_heap_expr h₁,
+   p ← to_expr ``(part_eq_parts_app_of_parts_parts %%p₀ %%p₁),
+   return (hs₀ ++ hs₁,p)
+ | e := fail "expecting expression of the form `part ?m ?m`"
+
+#print option.no_confusion_type
+
+meta def flatten_heap : tactic unit :=
+do t ← target,
+   (e₀,e₁) ← expr.is_eq t,
+   (ls,p) ← flat_heap_expr e₁,
+   h ← note `h none p,
+   `[simp at h],
+   asrt ← to_expr ``(some %%e₀ = some %%e₁),
+   h' ← assert `h asrt,
+   tactic.swap,
+   tactic.injection h' >> assumption,
+   h ← get_local `h,
+   rewrite_target h,
+   tactic.clear h,
+   return ()
+
+meta def eq_heap : tactic unit := do
+do t ← target,
+   (e₀, e₁) ← expr.is_eq t,
+   (_,p₀) ← flat_opt_heap_expr e₀,
+   (_,p₁) ← flat_opt_heap_expr e₁,
+   rewrite_target p₀,
+   rewrite_target p₁,
+   `[apply parts_congr, simp],
+   prove_perm
+
+#check perm
+
+section
+
+variables {hp hp₀ hp₁ hp₂ hp₃ : heap}
+variables (d₀₁ : hp₀ ## hp₁)
+variables (d₁₀ : hp₁ ## hp₀)
+variables (d₂₃ : hp₂ ## hp₃)
+variables (d₀₁₂₃ : disjoint (part' hp₀ hp₁ d₀₁) (part' hp₂ hp₃ d₂₃))
+variables (h : some hp = parts [hp₀,hp₁,hp₂,hp₃])
+include d₀₁ d₁₀ d₂₃ d₀₁₂₃ h
+example : hp = part' (part' hp₀ hp₁) (part' hp₂ hp₃) d₀₁₂₃ :=
+begin
+  flatten_heap,
+  apply h,
+end
+
+example : part  (part' hp₁ hp₀) (part' hp₂ hp₃) = part (part' hp₂ hp₃) (part' hp₀ hp₁)  :=
+begin
+  eq_heap
+end
+end
+
+end tactic.interactive
